Split constants into constants and c_constants

theories/CertiGC/model/constants.v
@@ -1,22 +1,7 @@
-From VST Require Import floyd.proofauto.
+From Coq Require Import micromega.Lia.
+From Coq Require Import ZArith.ZArith.
 
-Definition WORD_SIZE: Z
- := Eval cbv [Archi.ptr64]
- in if Archi.ptr64 then 8 else 4.
-Definition WORD_SIZE_pos: 0 < WORD_SIZE := eq_refl.
-
-Definition MAX_UINT: Z
- := Eval cbv [Archi.ptr64]
- in if Archi.ptr64 then Int64.max_unsigned else Int.max_unsigned.
-
-Definition MAX_SPACE_SIZE: Z
- := Eval cbv [Archi.ptr64]
- in if Archi.ptr64 then Z.shiftl 1 40 else Z.shiftl 1 29.
-
-Definition SPACE_STRUCT_SIZE: Z
- := Eval cbv [Archi.ptr64]
- in if Archi.ptr64 then 32 else 16.
-
+Local Open Scope Z.
 
 Definition MAX_SPACES: Z := 12.
 Definition MAX_SPACES_eq: MAX_SPACES = 12 := eq_refl.
@@ -30,22 +15,39 @@ Global Opaque NURSERY_SIZE.
 
 Definition generation_size (n: nat) := (NURSERY_SIZE * two_p (Z.of_nat n))%Z.
 
-Lemma generation_size_le_S: forall n : nat, generation_size n <= generation_size (S n).
+Lemma generation_size_le_S (n: nat): generation_size n <= generation_size (S n).
 Proof.
-    intros n. unfold generation_size. rewrite Nat2Z.inj_succ, two_p_S by lia.
-    assert (two_p (Z.of_nat n) > 0) by (apply two_p_gt_ZERO; lia).
-    assert (0 < NURSERY_SIZE) by (vm_compute; reflexivity).
-    rewrite Z.mul_assoc, (Z.mul_comm NURSERY_SIZE 2).
-    assert (0 < NURSERY_SIZE * two_p (Z.of_nat n)). apply Z.mul_pos_pos; lia.
-    rewrite <- Z.add_diag, Z.mul_add_distr_r. lia.
+  unfold generation_size.
+  rewrite Nat2Z.inj_succ, two_p_S by lia.
+  assert
+    (two_p (Z.of_nat n) > 0)
+    as H
+    by (apply two_p_gt_ZERO; lia).
+  assert
+    (0 < NURSERY_SIZE)
+    as H0
+    by easy.
+  rewrite Z.mul_assoc, (Z.mul_comm NURSERY_SIZE 2).
+  assert
+    (0 < NURSERY_SIZE * two_p (Z.of_nat n))
+    as H1
+    by (apply Z.mul_pos_pos; lia).
+  rewrite <- Z.add_diag, Z.mul_add_distr_r.
+  lia.
 Qed.
 
-Lemma ngs_0_lt: forall i, 0 < generation_size i.
+Lemma ngs_0_lt (i: nat): 0 < generation_size i.
 Proof.
-    intros. unfold generation_size.
-    rewrite NURSERY_SIZE_eq, Zbits.Zshiftl_mul_two_p, Z.mul_1_l,
-    <- two_p_is_exp by lia.
-    cut (two_p (16 + Z.of_nat i) > 0); [|apply two_p_gt_ZERO]; lia.
+  unfold generation_size.
+  rewrite NURSERY_SIZE_eq.
+  remember
+    (Z.of_nat i)
+    as z eqn:Heqz.
+  unfold two_p.
+  simpl Z.shiftl.
+  destruct z as [|z|z] ; try lia.
+  unfold two_power_pos.
+  lia.
 Qed.
 
 
@@ -58,37 +60,3 @@ Definition NO_SCAN_TAG: Z := 251.
 Definition NO_SCAN_TAG_eq: NO_SCAN_TAG = 251 := eq_refl.
 #[global]Hint Rewrite NO_SCAN_TAG_eq: rep_lia.
 Global Opaque NO_SCAN_TAG.
-
-
-Lemma four_div_WORD_SIZE: (4 | WORD_SIZE).
-Proof. first [now exists 1 | now exists 2]. Qed.
-
-Definition MSS_eq_unsigned: Int.unsigned (Int.shl (Int.repr 1) (Int.repr 29)) = Z.shiftl 1 29 := eq_refl.
-
-Lemma MSS_max_unsigned_range (n: Z) (Hn: 0 <= n < MAX_SPACE_SIZE):
-    0 <= n <= MAX_UINT.
-Proof.
-    split ; try lia.
-    now transitivity MAX_SPACE_SIZE ; try lia.
-Qed.
-
-Lemma MSS_max_wordsize_unsigned_range (n: Z) (Hn: 0 <= n < MAX_SPACE_SIZE):
-    0 <= WORD_SIZE * n <= MAX_UINT.
-Proof.
-    pose proof WORD_SIZE_pos as HH.
-    split ; try lia.
-    now transitivity (WORD_SIZE * MAX_SPACE_SIZE) ; try nia.
-Qed.
-
-Lemma MSS_max_wordsize_signed_range (n: Z) (Hn: 0 <= n < MAX_SPACE_SIZE):
-    Ptrofs.min_signed <= WORD_SIZE * n <= Ptrofs.max_signed.
-Proof.
-  destruct Hn as [Hn_lo Hn_hi].
-  split.
-  - unfold WORD_SIZE.
-    transitivity 0 ; now try lia.
-  - rewrite Z.le_lteq.
-    left.
-    rewrite Z.lt_le_pred in Hn_hi.
-    apply Z.le_lt_trans with (WORD_SIZE * Z.pred MAX_SPACE_SIZE) ; unfold WORD_SIZE ; now try lia.
-Qed.
