theories/CertiGC/model/heapgraph/block/cell.v
@@ -7,7 +7,7 @@ From CertiGraph Require Import graph.graph_model.
 From CertiGraph Require Import lib.List_ext.
 
 From CertiGC Require Import model.heapgraph.block.block.
-From CertiGC Require Import model.heapgraph.block.block_rep.
+From CertiGC Require Import model.heapgraph.block.ptr.
 From CertiGC Require Import model.heapgraph.generation.generation.
 From CertiGC Require Import model.heapgraph.graph.
 From CertiGC Require Import model.util.
