theories/CertiGC/model/op/garbage_collect.v
@@ -14,7 +14,7 @@ From CertiGC Require Import model.compatible.compatible.
 From CertiGC Require Import model.constants.
 From CertiGC Require Import model.heap.heap.
 From CertiGC Require Import model.heapgraph.block.block.
-From CertiGC Require Import model.heapgraph.block.block_rep.
+From CertiGC Require Import model.heapgraph.block.ptr.
 From CertiGC Require Import model.heapgraph.block.cell.
 From CertiGC Require Import model.heapgraph.block.field.
 From CertiGC Require Import model.heapgraph.field_pairs.
