theories/CertiGC/model/op/scan.v
@@ -12,7 +12,7 @@ From CertiGraph Require Import lib.List_ext.
 
 From CertiGC Require Import model.compatible.compatible.
 From CertiGC Require Import model.heapgraph.block.block.
-From CertiGC Require Import model.heapgraph.block.block_rep.
+From CertiGC Require Import model.heapgraph.block.ptr.
 From CertiGC Require Import model.heapgraph.block.cell.
 From CertiGC Require Import model.heapgraph.block.field.
 From CertiGC Require Import model.heapgraph.field_pairs.
